some work on the Imp compiler

src/coq/Compiler.v
@@ -1,8 +1,92 @@
+Require Import ZArith String Omega Lists Equalities MSets.
+
 (* Vellvm dependencies *)
-Require Import Vellvm.Classes.
+Require Import Vellvm.Classes Vellvm.Ollvm_ast Vellvm.AstLib.
 
 (* Logical Foundations dependencies *)
 Require Import Imp Maps.
+
+
+(* Auxilliary definitions for working with Identifiers ---------------------- *)
+
+Module IDDec <: MiniDecidableType.
+  Definition t := id.
+  Lemma eq_dec : forall (x y : t), {x = y} + {x <> y}.
+  Proof.
+    intros x y.
+    destruct x as [s]. destruct y as [t].
+    destruct (s == t); subst; auto.
+    right. unfold not. intros H. apply n. inversion H; auto.
+  Qed.
+End IDDec.
+Module ID := Make_UDT(IDDec).
+Instance eq_dec_id : eq_dec id := ID.eq_dec.
+
+Module IDSet := MSetWeakList.Make(ID).
+
+
+(* Free variable calculation ------------------------------------------------ *)
+
+Class FV X := fv : X -> IDSet.t.
+
+Fixpoint fv_aexp (a:aexp) : IDSet.t :=
+  match a with
+  | ANum _ => IDSet.empty
+  | AId x => IDSet.singleton x
+  | APlus a1 a2
+  | AMinus a1 a2
+  | AMult a1 a2 => IDSet.union (fv_aexp a1) (fv_aexp a2)
+  end.
+Instance FV_aexp : FV aexp := fv_aexp.
+
+Fixpoint fv_bexp (b:bexp) : IDSet.t :=
+  match b with
+  | BTrue | BFalse => IDSet.empty
+  | BEq a1 a2
+  | BLe a1 a2 => IDSet.union (fv a1) (fv a2)
+  | BNot b => fv_bexp b
+  | BAnd b1 b2 => IDSet.union (fv_bexp b1) (fv_bexp b2)
+  end.
+Instance FV_bexp : FV bexp := fv_bexp.
+
+Fixpoint fv_com (c:com) : IDSet.t :=
+  match c with
+  | CSkip => IDSet.empty
+  | CAss x a => IDSet.union (IDSet.singleton x) (fv a)
+  | CSeq c1 c2 => IDSet.union (fv_com c1) (fv_com c2)
+  | CIf b c1 c2 => IDSet.union (fv b) (IDSet.union (fv_com c1) (fv_com c2))
+  | CWhile b c => IDSet.union (fv b) (fv_com c)
+  end.
+Instance FV_com : FV com := fv_com.
+
+(* LLVM Identifier generation monad ----------------------------------------- *)
+
+Definition GenSym A := ST int A.
+Definition gensym : () -> GenSym (local_id) :=
+  fun _ => fun n => (1+n, Anon (n))%Z.
+
+
+(* A context maps Imp variables to Vellvm identifiers
+   Invariant: 
+      storage space for an Imp variable is represented as an alloca'ed 
+      ctxt (Id X) is the identifier for the pointer to the storage for X.
+
+*)
+Definition ctxt := partial_map ident.
+
+Inductive elt :=
+| L (lbl:block_id)
+| I (id:instr_id) (ins:instr)
+| T (id:instr_id) (t:terminator)
+.    
+
+
+
+
+
+
+
+
 
 
 
